Otway-Rees: implemented serialization of AuthServerSession and InitiatorInit states

otway-rees/OYRS.Sessions.fst
@@ -3,7 +3,7 @@ module OYRS.Sessions
 
 let valid_session i p si vi st =
   match st with
-  | AuthServerSession pri k_pri_srv -> is_labeled i k_pri_srv (readers [P pri; P p])
+  | AuthServerSession pri k_pri_srv -> MSG.is_msg i k_pri_srv (readers [P p])
   | InitiatorInit srv k_as b -> is_labeled i k_as (readers [P p; P srv])
   | ResponderInit srv k_bs -> is_labeled i k_bs (readers [P p; P srv])
   | InitiatorSentMsg1 srv k_as b c n_a ->
@@ -12,12 +12,30 @@ let valid_session i p si vi st =
     is_labeled i n_a (readers [P p; P srv])
   | ResponderSentMsg2 srv k_bs a c n_b ->
     is_labeled i k_bs (readers [P p; P srv]) /\
-    is_labeled i c public /\
+    MSG.is_msg i c public /\
     is_labeled i n_b (readers [P p; P srv])
   | AuthServerSentMsg3 a b c n_a n_b k_ab ->
-    is_labeled i c public /\
-    is_labeled i n_a (readers [P a; P p]) /\
-    is_labeled i n_b (readers [P b; P p]) /\
+    MSG.is_msg i c public /\
+    MSG.is_msg i n_a (readers [P p]) /\
+    MSG.is_msg i n_b (readers [P p]) /\
     is_labeled i k_ab (readers [P p; P a; P b])
-  | ResponderSentMsg4 srv a k_ab -> is_labeled i k_ab (readers [P srv; P a; P p])
-  | InitiatorRecvedMsg4 srv b k_ab -> is_labeled i k_ab (readers [P srv; P p; P b])
+  | ResponderSentMsg4 srv a k_ab -> MSG.is_msg i k_ab (readers [P p])
+  | InitiatorRecvedMsg4 srv b k_ab -> MSG.is_msg i k_ab (readers [P p])
+
+let serialize_session_st i p si vi st =
+  match st with
+  | AuthServerSession pri k_pri_srv ->
+    let tag = str_to_bytes #i "auth_srv_sess" in
+    let pri_bytes = str_to_bytes #i pri in
+    let _ = assert(valid_session i p si vi st) in
+    let _ = assert(MSG.is_msg i k_pri_srv (readers [P p])) in
+    LC.can_flow_transitive i (LC.get_label MSG.oyrs_key_usages k_pri_srv) (readers [P p]) (readers [V p si vi]);
+    // TODO: why assert needed??
+    let _ = assert(MSG.is_msg i k_pri_srv (readers [V p si vi])) in
+    concat #i #(readers [V p si vi]) tag (concat #i #(readers [V p si vi]) pri_bytes k_pri_srv)
+  | InitiatorInit srv k_as b ->
+    let tag = str_to_bytes #i "i_init" in
+    let srv_bytes = str_to_bytes #i srv in
+    let b_bytes = str_to_bytes #i b in
+    concat #i #(readers [V p si vi]) tag (concat #i #(readers [V p si vi]) srv_bytes (concat #i #(readers [V p si vi]) k_as b_bytes))
+  | _ -> admit()
